program-schedule-encoding/reverse-list-get-write.v
@@ -1,0 +1,20 @@
+Require Import Omega.
+
+Inductive revlist: nat ->  Type :=
+| CSeq: forall (n: nat), revlist n -> nat -> revlist (n + 1)
+| CBegin: revlist 0.
+
+(* Reasoning about this definition is impossible, because when "omega" usage leads to unreadable definitions of getNatAt inside proofs *)
+
+Fixpoint getNatAt (n: nat) (c: revlist n) (i: nat) (witness_ub: i <= n) (witness_lb: i >= 1)  :=
+  match c in (revlist n) return (i <= n -> i >= 1 -> nat) with
+  | CBegin => fun E1 E2 => 0
+  | CSeq n' c' curval => fun E1 E2 => 1
+  end.
+
+
+  (* Now what? how do I reason about the relationship between n and i? *)
+Abort.
+
+ 
+(* How do I write the same thing with dependent type style + actual computation, not tactic / proof based? *)
